first cut at starting PivotBetreeSpec

disk-betree/MapSpec.dfy
@@ -1,9 +1,11 @@
 include "../tla-tree/MissingLibrary.dfy"
+include "../lib/total_order.dfy"
 
 module MapSpec {
 import opened MissingLibrary
 
-type Key(!new,==)
+import Keyspace = Total_Order
+type Key = Keyspace.Element
 
 // Users must provide a definition of EmptyValue
 function EmptyValue<Value>() : Value
