disk-betree/PivotBetreeSpec.dfy
@@ -1,0 +1,353 @@
+include "BlockInterface.dfy"  
+include "../lib/sequences.dfy"
+include "../lib/Maps.dfy"
+include "MapSpec.dfy"
+include "Graph.dfy"
+include "../tla-tree/MissingLibrary.dfy"
+
+module PivotBetreeGraph refines Graph {
+  import MS = MapSpec
+  import opened MissingLibrary
+
+  import Keyspace = MS.Keyspace
+  type Key = Keyspace.Element
+  type Value(!new)
+
+  datatype BufferEntry = Insertion(value: Value) // TODO duplication
+
+  datatype PivotTable = PivotTable(pivots: seq<Key>)
+  datatype BufferPair = BufferPair(key: Key, entry: BufferEntry)
+
+  datatype Bucket = Bucket(
+      child: Option<Reference>,
+      buffer: seq<BufferPair>)
+
+  datatype Node = Node(
+      pivotTable: PivotTable,
+      buckets: seq<Bucket>)
+
+  function Successors(node: Node) : iset<Reference>
+  {
+    iset i | 0 <= i < |node.buckets| && node.buckets[i].child.Some? :: node.buckets[i].child.value
+  }
+}
+
+module PivotBetreeSpec {
+  import MS = MapSpec
+  import opened G = PivotBetreeGraph
+  import opened Sequences
+  import opened Maps
+  import opened MissingLibrary
+
+  export Spec provides BetreeStep, ValidBetreeStep, BetreeStepReads, BetreeStepOps, G
+  export Internal reveals *
+
+  export extends Spec // Default export-style is Spec
+
+  function PivotTableSize(pivotTable: PivotTable) : int
+  {
+    |pivotTable.pivots| + 1
+  }
+
+  predicate WFPivotTable(pivotTable: PivotTable)
+  {
+    Keyspace.IsStrictlySorted(pivotTable.pivots)
+  }
+
+  function Route(pivotTable: PivotTable, key: Key) : int
+  requires WFPivotTable(pivotTable)
+  {
+    Keyspace.LargestLte(pivotTable.pivots, key) + 1
+  }
+
+  predicate WFNode(node: Node)
+  {
+    && PivotTableSize(node.pivotTable) == |node.buckets|
+    && WFPivotTable(node.pivotTable)
+    && (|node.buckets| > 1 ==> forall i | 0 <= i < |node.buckets| :: node.buckets[i].child.Some?)
+  }
+
+  // Adding messages to buffers
+
+  function AddMessageToNode(node: Node, key: Key, msg: BufferEntry) : Node
+  requires WFNode(node)
+  ensures WFNode(AddMessageToNode(node, key, msg))
+  {
+    node.(
+      buckets := node.buckets[
+        Route(node.pivotTable, key) := Bucket(
+          node.buckets[Route(node.pivotTable, key)].child,
+          [BufferPair(key, msg)] + node.buckets[Route(node.pivotTable, key)].buffer
+        )
+      ]
+    )
+  }
+
+  function AddMessagesToNode(node: Node, pairs: seq<BufferPair>) : Node
+  requires WFNode(node)
+  {
+    if |pairs| == 0 then (
+      node
+    ) else (
+      AddMessageToNode(AddMessagesToNode(node, pairs[1..]), pairs[0].key, pairs[0].entry)
+    )
+  }
+
+  //// Insert
+
+  datatype MessageInsertion = MessageInsertion(key: Key, msg: BufferEntry, oldroot: Node)
+
+  predicate ValidInsertion(ins: MessageInsertion) {
+    && WFNode(ins.oldroot)
+  }
+
+  function InsertionReads(ins: MessageInsertion): seq<ReadOp>
+  requires ValidInsertion(ins)
+  {
+    [G.ReadOp(Root(), ins.oldroot)]
+  }
+
+  function InsertionOps(ins: MessageInsertion) : seq<Op>
+  requires ValidInsertion(ins)
+  {
+    var newroot := AddMessageToNode(ins.oldroot, ins.key, ins.msg);
+    var writeop := G.WriteOp(Root(), newroot);
+    [writeop]
+  }
+
+  //// Flush
+
+  datatype NodeFlush = NodeFlush(parentref: Reference, parent: Node, childref: Reference, child: Node, newchildref: Reference, slotIndex: int)
+
+  predicate ValidFlush(flush: NodeFlush)
+  {
+    && WFNode(flush.parent)
+    && WFNode(flush.child)
+    && 0 <= flush.slotIndex < |flush.parent.buckets|
+    && flush.parent.buckets[flush.slotIndex].child == Some(flush.childref)
+  }
+
+  function FlushReads(flush: NodeFlush) : seq<ReadOp>
+  requires ValidFlush(flush)
+  {
+    [
+      G.ReadOp(flush.parentref, flush.parent),
+      G.ReadOp(flush.childref, flush.child)
+    ]
+  }
+
+  function FlushOps(flush: NodeFlush) : seq<Op>
+  requires ValidFlush(flush)
+  {
+    var newparent := flush.parent.(buckets := flush.parent.buckets[flush.slotIndex := Bucket(Some(flush.newchildref), [])]);
+    var newchild := AddMessagesToNode(flush.child, flush.parent.buckets[flush.slotIndex].buffer);
+    var allocop := G.AllocOp(flush.newchildref, newchild);
+    var writeop := G.WriteOp(flush.parentref, newparent);
+    [allocop, writeop]
+  }
+
+  //// Grow
+
+  datatype RootGrowth = RootGrowth(oldroot: Node, newchildref: Reference)
+
+  predicate ValidGrow(growth: RootGrowth)
+  {
+    true
+  }
+
+  function GrowReads(growth: RootGrowth) : seq<ReadOp>
+  requires ValidGrow(growth)
+  {
+    [G.ReadOp(Root(), growth.oldroot)]
+  }
+
+  function GrowOps(growth: RootGrowth) : seq<Op>
+  requires ValidGrow(growth)
+  {
+    var newroot := Node(PivotTable([]), [Bucket(Some(growth.newchildref), [])]);
+    var allocop := G.AllocOp(growth.newchildref, growth.oldroot);
+    var writeop := G.WriteOp(Root(), newroot);
+    [allocop, writeop]
+  }
+
+  //// Split
+
+  datatype NodeFusion = NodeFusion(
+    parentref: Reference,
+    fused_childref: Reference,
+    left_childref: Reference,
+    right_childref: Reference,
+    fused_parent: Node,
+    split_parent: Node,
+    fused_child: Node,
+    left_child: Node,
+    right_child: Node,
+    
+    slot_idx: int
+  )
+
+  predicate BufferFusion(
+      fusedBuffer: seq<BufferPair>,
+      leftBuffer: seq<BufferPair>,
+      rightBuffer: seq<BufferPair>,
+      pivot: Key)
+  {
+    if |fusedBuffer| == 0 then
+      |leftBuffer| == 0 && |rightBuffer| == 0
+    else (
+      var key := fusedBuffer[0].key;
+      if Keyspace.lt(key, pivot) then (
+        && |leftBuffer| > 0
+        && leftBuffer[0] == fusedBuffer[0]
+        && BufferFusion(fusedBuffer[1..], leftBuffer[1..], rightBuffer, pivot)
+      ) else (
+        && |rightBuffer| > 0
+        && rightBuffer[0] == rightBuffer[0]
+        && BufferFusion(fusedBuffer[1..], leftBuffer, rightBuffer[1..], pivot)
+      )
+    )
+  }
+
+  predicate PivotTableFusion(table: PivotTable, left: PivotTable, right: PivotTable, pivot: Key)
+  {
+    && table.pivots == concat3(left.pivots, pivot, right.pivots)
+  }
+
+  predicate ChildFusion(child: Node, left: Node, right: Node, pivot: Key)
+  {
+    && left.buckets + right.buckets == child.buckets
+    && PivotTableFusion(child.pivotTable, left.pivotTable, right.pivotTable, pivot)
+  }
+
+  predicate ValidFusion(fusion: NodeFusion)
+  {
+    && WFNode(fusion.split_parent)
+    && WFNode(fusion.fused_parent)
+
+    && 0 <= fusion.slot_idx < |fusion.fused_parent.buckets|
+    && |fusion.split_parent.buckets| == |fusion.fused_parent.buckets| + 1
+
+    && fusion.fused_parent.buckets[fusion.slot_idx].child == Some(fusion.fused_childref)
+    && fusion.split_parent.buckets[fusion.slot_idx].child == Some(fusion.left_childref)
+    && fusion.split_parent.buckets[fusion.slot_idx + 1].child == Some(fusion.right_childref)
+    && BufferFusion(
+        fusion.fused_parent.buckets[fusion.slot_idx].buffer,
+        fusion.split_parent.buckets[fusion.slot_idx].buffer,
+        fusion.split_parent.buckets[fusion.slot_idx + 1].buffer,
+        fusion.split_parent.pivotTable.pivots[fusion.slot_idx])
+
+    && (forall i | 0 < i < fusion.slot_idx :: fusion.fused_parent.buckets[i] == fusion.split_parent.buckets[i])
+    && (forall i | fusion.slot_idx < i < |fusion.fused_parent.buckets| :: fusion.fused_parent.buckets[i] == fusion.split_parent.buckets[i+1])
+
+    && (forall i | 0 < i < fusion.slot_idx ::
+        fusion.fused_parent.pivotTable.pivots[i] == fusion.split_parent.pivotTable.pivots[i])
+    && (forall i | fusion.slot_idx < i < |fusion.fused_parent.pivotTable.pivots| ::
+        fusion.fused_parent.pivotTable.pivots[i] == fusion.split_parent.pivotTable.pivots[i+1])
+
+    && ChildFusion(
+        fusion.fused_child,
+        fusion.left_child,
+        fusion.right_child,
+        fusion.split_parent.pivotTable.pivots[fusion.slot_idx])
+  }
+
+  predicate ValidSplit(fusion: NodeFusion)
+  {
+    && WFNode(fusion.fused_parent)
+    && WFNode(fusion.fused_child)
+    && WFNode(fusion.left_child)
+    && WFNode(fusion.right_child)
+    && ValidFusion(fusion)
+  }
+
+  function SplitReads(fusion: NodeFusion) : seq<ReadOp>
+  requires ValidSplit(fusion)
+  {
+    [
+      ReadOp(fusion.parentref, fusion.fused_parent),
+      ReadOp(fusion.fused_childref, fusion.fused_child)
+    ]
+  }
+
+  function SplitOps(fusion: NodeFusion) : seq<Op>
+  requires ValidSplit(fusion)
+  {
+    [
+      G.AllocOp(fusion.left_childref, fusion.left_child),
+      G.AllocOp(fusion.right_childref, fusion.right_child),
+      G.WriteOp(fusion.parentref, fusion.split_parent)
+    ]
+  }
+
+  //// Merge
+
+  predicate ValidMerge(fusion: NodeFusion)
+  {
+    ValidFusion(fusion)
+  }
+
+  function MergeReads(fusion: NodeFusion) : seq<ReadOp>
+  requires ValidMerge(fusion)
+  {
+    [
+      ReadOp(fusion.parentref, fusion.split_parent),
+      ReadOp(fusion.left_childref, fusion.left_child),
+      ReadOp(fusion.right_childref, fusion.right_child)
+    ]
+  }
+
+  function MergeOps(fusion: NodeFusion) : seq<Op>
+  requires ValidMerge(fusion)
+  {
+    [
+      G.AllocOp(fusion.fused_childref, fusion.fused_child),
+      G.WriteOp(fusion.parentref, fusion.fused_parent)
+    ]
+  }
+
+
+  //// Put it all together
+
+  datatype BetreeStep =
+    | BetreeInsert(ins: MessageInsertion)
+    | BetreeFlush(flush: NodeFlush)
+    | BetreeGrow(growth: RootGrowth)
+    | BetreeSplit(fusion: NodeFusion)
+    | BetreeMerge(fusion: NodeFusion)
+
+  predicate ValidBetreeStep(step: BetreeStep)
+  {
+    match step {
+      case BetreeInsert(ins) => ValidInsertion(ins)
+      case BetreeFlush(flush) => ValidFlush(flush)
+      case BetreeGrow(growth) => ValidGrow(growth)
+      case BetreeSplit(fusion) => ValidSplit(fusion)
+      case BetreeMerge(fusion) => ValidMerge(fusion)
+    }
+  }
+
+  function BetreeStepReads(step: BetreeStep) : seq<ReadOp>
+  requires ValidBetreeStep(step)
+  {
+    match step {
+      case BetreeInsert(ins) => InsertionReads(ins)
+      case BetreeFlush(flush) => FlushReads(flush)
+      case BetreeGrow(growth) => GrowReads(growth)
+      case BetreeSplit(fusion) => SplitReads(fusion)
+      case BetreeMerge(fusion) => MergeReads(fusion)
+    }
+  }
+
+  function BetreeStepOps(step: BetreeStep) : seq<Op>
+  requires ValidBetreeStep(step)
+  {
+    match step {
+      case BetreeInsert(ins) => InsertionOps(ins)
+      case BetreeFlush(flush) => FlushOps(flush)
+      case BetreeGrow(growth) => GrowOps(growth)
+      case BetreeSplit(fusion) => SplitOps(fusion)
+      case BetreeMerge(fusion) => MergeOps(fusion)
+    }
+  }
+
+}
